make parsers aware of the tagging system, get rid of dynamic typing

ParserCombinators/Memoized.lean
@@ -8,11 +8,12 @@ import Std.Data.HashMap.Lemmas
 import Mathlib.Control.Traversable.Basic
 import Mathlib.Control.Fold
 import ParserCombinators.MState
+import ParserCombinators.Util
 import Aesop
 
 -- β is the alphabet: parsers work over Array β
 universe u v
-variable { α β : Type u } { μ : Type u → Type u } [BEq β]
+variable {τ} { α β : Type u } {tag : τ → Type u} { μ : Type u → Type u } [BEq β] [BEq τ] [LawfulBEq τ] [Hashable τ]
 
 -- Tags for each parser, these don't carry type information.
 --
@@ -24,75 +25,56 @@ structure Tag where
   id : Int
   deriving DecidableEq, BEq, Hashable
 
-structure MemoData : Type v where
-  nextTag : Int -- need only the data inside
-  table : Std.HashMap Tag (Std.HashMap Int Dynamic)
-
-instance : SemilatticeSup MemoData := sorry
-
-def startState : MemoData := {
-  nextTag := 0
-  table := Std.HashMap.emptyWithCapacity
+def startState {μ} [CollectionLike μ] : MemoData tag μ := {
+  table := Std.DHashMap.emptyWithCapacity
 }
 
 abbrev UChar := ULift Char
 abbrev UString := ULift String
 
-namespace Std.HashMap
-def unionWith {K V} [BEq K] [Hashable K] (m1 m2 : Std.HashMap K V) (f : V → V → V) : Std.HashMap K V :=
-  m2.fold (fun m k v2 =>
-    match m[k]? with
-    -- Collision case, meshes the two values found into one new value (based on the given function `f`)
-    | some v1 => m.insert k (f v1 v2)
-    -- New key case, juar adds the value we found
-    | none => m.insert k v2) m1
-end Std.HashMap
-
 @[inline]
 def liftA2 {F : Type u → Type v} [Applicative F] {α β γ : Type u} (f : α → β → γ) (fa : F α) (fb : F β) : F γ :=
   f <$> fa <*> fb
 
-def joinUnderCache {β γ} [Monad μ] [Alternative μ] (s1 s2 : MStateT MemoData (ReaderM (Array β)) (Std.HashMap Int (μ γ))) : MStateT MemoData (ReaderM (Array β)) (Std.HashMap Int (μ γ)) :=
+def joinUnderCache {γ} [CollectionLike μ] (s1 s2 : MStateT (MemoData tag μ) (ReaderM (Array β)) (Std.HashMap Int (μ γ)))
+    : MStateT (MemoData tag μ) (ReaderM (Array β)) (Std.HashMap Int (μ γ)) :=
   liftA2 (fun m1 m2 => Std.HashMap.unionWith m1 m2 (fun v1 v2 => v1 <|> v2)) s1 s2
 
-abbrev ParserState (μ : Type u → Type u) [Monad μ] (α : Type u) :=
-  MStateT MemoData (ReaderM (Array β)) (Std.HashMap Int (μ α))
-
 -- Some of the α's here should become existential/hidden
-abbrev Parser (β : Type u) (μ : Type u → Type u) [Monad μ] (α : Type u) :=
-  Int → MStateT MemoData (ReaderM (Array β)) (Std.HashMap Int (μ α))
+abbrev Parser (β : Type u) (μ : Type u → Type u) [CollectionLike μ] (α : Type u) :=
+  Int → MStateT (MemoData tag μ) (ReaderM (Array β)) (Std.HashMap Int (μ α))
 
-instance [Monad μ] : Functor (Parser β μ) where
+instance [CollectionLike μ] : Functor (Parser (tag := tag) β μ) where
   map f x := Functor.map (Std.HashMap.map (fun _ => Functor.map f)) ∘ x
 
 -- N.B. Have to define `pure` separately so that we can use it in `seq`
 -- Defines the ability to create the simplest parser possible
-instance [Monad μ] : Pure (Parser β μ) where
+instance [CollectionLike μ] : Pure (Parser (tag := tag) β μ) where
   pure a := fun pos => pure {(pos, pure a)}
 
 -- might need other type class instances (e.g. to make fold work)
 -- also, you may need to define or find a fold operation for Std.HashMap
-instance [Monad μ] [Alternative μ] [Traversable μ] : Bind (Parser β μ) where
+instance [CollectionLike μ] [Traversable μ] : Bind (Parser (tag := tag) β μ) where
   bind {_ β'} x f := fun pos => do
       let pivotToResult ← x pos
-      let actions : List (μ (MStateT MemoData (ReaderM (Array β)) (Std.HashMap Int (μ β')))) :=
+      let actions : List (μ (MStateT (MemoData tag μ) (ReaderM (Array β)) (Std.HashMap Int (μ β')))) :=
         pivotToResult.toList.map (fun (j, ma) => (fun a => f a j) <$> ma)
       actions.foldl
         (Traversable.foldl joinUnderCache)
         (pure Std.HashMap.emptyWithCapacity)
 
-instance [Monad μ] [Alternative μ] [Traversable μ] : Monad (Parser β μ) where
+instance [CollectionLike μ] [Traversable μ] : Monad (Parser (tag := tag) β μ) where
 
-instance [Monad μ] [Alternative μ] [Traversable μ] : Alternative (Parser β μ) where
+instance [CollectionLike μ] [Traversable μ] : Alternative (Parser (tag := tag) β μ) where
   failure _pos := pure Std.HashMap.emptyWithCapacity
   orElse r1 r2 pos :=
     let s1 := r1 pos
     let s2 := r2 () pos
     joinUnderCache s1 s2
 
-def epsilon [Monad μ] : Parser β μ PUnit := fun pos => pure {(pos, pure $ PUnit.unit)}
+def epsilon [CollectionLike μ] : Parser (tag := tag) β μ PUnit := fun pos => pure {(pos, pure $ PUnit.unit)}
 
-def terminal [Monad μ] [Alternative μ] (s : String) : Parser UChar μ UString := fun pos => do
+def terminal [CollectionLike μ] (s : String) : Parser (tag := tag) UChar μ UString := fun pos => do
   let input ← read
   if pos >= 0 && (s.data.map ULift.up).toArray.isPrefixOf (input.extract pos.toNat) then
     let endPos := pos + s.length
@@ -100,14 +82,15 @@ def terminal [Monad μ] [Alternative μ] (s : String) : Parser UChar μ UString 
   else
     pure Std.HashMap.emptyWithCapacity
 
-def terminal' [Monad μ] [Alternative μ] (t: β) : Parser β μ β := fun pos => do
+def terminal' [CollectionLike μ] (t: β) : Parser (tag := tag) β μ β := fun pos => do
   let input ← read
   if pos >= 0 && some t == input[pos.toNat]? then
     pure {(pos + 1, pure t)}
   else
     pure Std.HashMap.emptyWithCapacity
 
-def memoize [TypeName α] [Monad μ] [TypeName (μ α)] (tag : Tag) (p : Parser β μ α) : Parser β μ α :=
+/-
+def memoize [TypeName α] [CollectionLike μ] [TypeName (μ α)] (tag : Tag) (p : Parser (tag := tag) β μ α) : Parser (tag := tag) β μ α :=
   fun pos => do
     let memo ← get
     -- Check if we have cached results for this tag and position
@@ -145,112 +128,119 @@ def memoize [TypeName α] [Monad μ] [TypeName (μ α)] (tag : Tag) (p : Parser 
       let newTable := memo.table.insert tag newPositionMap
       set { memo with table := newTable }
       pure results
+-/
 
 -- Testing
 
 -- Will use `Option` as the concrete monad (some is success and none is failure)
 
-def runParser [Monad μ] (p : Parser β μ α) (input : Array β) (pos : Int := 0) : (Std.HashMap Int (μ α)) × MemoData :=
+def runParser [CollectionLike μ] (p : Parser (tag := tag) β μ α) (input : Array β) (pos : Int := 0) : (Std.HashMap Int (μ α)) × MemoData tag μ :=
   let stateTResult := (p pos).run startState
   let readerResult := stateTResult.run input
   readerResult
 
-def runParser' [Monad μ] (p : Parser UChar μ α) (input : String) (pos : Int := 0) : (Std.HashMap Int (μ α)) × MemoData :=
+def runParser' [CollectionLike μ] (p : Parser (tag := tag) UChar μ α) (input : String) (pos : Int := 0) : (Std.HashMap Int (μ α)) × MemoData tag μ :=
   runParser p (input.toList.map ULift.up).toArray pos
 
+def emptyTag : PUnit → Type := fun _ => PUnit
+
+def runParserO {μ : Type → Type} {α : Type} [CollectionLike μ]
+  (p : Parser (tag := emptyTag) UChar μ α) (input : String) (pos : Int := 0)
+    : (Std.HashMap Int (μ α)) × MemoData emptyTag μ :=
+  runParser'.{0} p input pos
 
 -- Checking to make sure that runParser has correct type
-#guard (runParser'.{0} (μ := Option) epsilon "test").1.toList == [(0, some PUnit.unit)]
+#guard (runParserO (μ := Option) epsilon "test").1.toList == [(0, some PUnit.unit)]
 
 -- Testing running the parsers (had to extract just the hashmap
 -- because Lean couldn't extract a string from the full return type)
-#guard (runParser'.{0} (μ := Option) (terminal "hello") "hello world").1.toList == [(5, some $ ULift.up "hello")]
-#guard (runParser'.{0} (μ := Option) (terminal "wo") "hello world" 6).1.toList == [(8, some $ ULift.up "wo")]
+#guard (runParserO (μ := Option) (terminal "hello") "hello world").1.toList == [(5, some $ ULift.up "hello")]
+#guard (runParserO (μ := Option) (terminal "wo") "hello world" 6).1.toList == [(8, some $ ULift.up "wo")]
 
 -- Failure
-#guard (runParser'.{0} (μ := Option) (terminal "llo") "hello world" 5).1.isEmpty
+#guard (runParserO (μ := Option) (terminal "llo") "hello world" 5).1.isEmpty
 
 -- Edge case for empty string
-#guard (runParser'.{0} (μ := Option) (terminal "") "hello world" 6).1.toList == [(6, some $ ULift.up "")]
+#guard (runParserO (μ := Option) (terminal "") "hello world" 6).1.toList == [(6, some $ ULift.up "")]
 
 
 -- Testing instances:
 
 -- Functor (`<$>`)
-def funcParser : Parser UChar Option String := (fun _ => "matched!") <$> terminal "hello"
-def funcParser2 : Parser UChar Option Int := (fun x => x * 3) <$> terminal "hello" $> 2
+def funcParser : Parser (tag := emptyTag) UChar Option String := (fun _ => "matched!") <$> terminal "hello"
+def funcParser2 : Parser (tag := emptyTag) UChar Option Int := (fun x => x * 3) <$> terminal "hello" $> 2
 
 -- TODO: (Madi) Just beef this up by testing edge cases
-#guard (runParser' (μ := Option) funcParser "hello world").1.toList == [(5, some "matched!")]
-#guard (runParser' (μ := Option) funcParser "hell").1.toList == []
-#guard (runParser' (μ := Option) funcParser2 "hello").1.toList == [(5, some 6)]
+#guard (runParserO (μ := Option) funcParser "hello world").1.toList == [(5, some "matched!")]
+#guard (runParserO (μ := Option) funcParser "hell").1.toList == []
+#guard (runParserO (μ := Option) funcParser2 "hello").1.toList == [(5, some 6)]
 
 -- Alternative (`<|>`)
-def altParser [Monad μ] [Alternative μ] [Traversable μ] : Parser  UChar μ UString :=
+def altParser [CollectionLike μ] [Traversable μ] : Parser (tag := tag) UChar μ UString :=
   terminal "hello" <|> terminal "goodbye"
 
-#guard (runParser'.{0} (μ := Option) altParser "hello").1.toList == [(5, some $ ULift.up "hello")]
-#guard (runParser'.{0} (μ := Option) altParser "goodbye").1.toList == [(7, some $ ULift.up "goodbye")]
-#guard (runParser'.{0} (μ := List) altParser "hello").1.toList == [(5, [ULift.up "hello"])]
-#guard (runParser'.{0} (μ := List) altParser "goodbye").1.toList == [(7, [ULift.up "goodbye"])]
+#guard (runParserO (μ := Option) altParser "hello").1.toList == [(5, some $ ULift.up "hello")]
+#guard (runParserO (μ := Option) altParser "goodbye").1.toList == [(7, some $ ULift.up "goodbye")]
+#guard (runParserO (μ := List) altParser "hello").1.toList == [(5, [ULift.up "hello"])]
+#guard (runParserO (μ := List) altParser "goodbye").1.toList == [(7, [ULift.up "goodbye"])]
 
 -- Concatenation via bind (`>>=`)
-def concatParser {μ : Type → Type} [Monad μ] [Alternative μ] [Traversable μ] : Parser UChar μ (Int × Int) :=
+def concatParser {μ : Type → Type} [CollectionLike μ] [Traversable μ] : Parser (tag := emptyTag) UChar μ (Int × Int) :=
   (terminal "hello" $> 1) >>= (fun a => terminal "goodbye" $> (a, 2))
 -- NOTE(maemre): the commented-out tests crash
-#guard (runParser'.{0} (μ := Option) concatParser "hello").1.toList == []
-#guard (runParser'.{0} (μ := Option) concatParser "goodbye").1.toList == []
-#guard (runParser'.{0} (μ := Option) concatParser "hellogoodbye").1.toList == [(12, some (1, 2))]
+#guard (runParserO (μ := Option) concatParser "hello").1.toList == []
+#guard (runParserO (μ := Option) concatParser "goodbye").1.toList == []
+#guard (runParserO (μ := Option) concatParser "hellogoodbye").1.toList == [(12, some (1, 2))]
 -- #guard (runParser.{0} (μ := List) concatParser "hello").1.toList == []
-#guard (runParser'.{0} (μ := List) concatParser "goodbye").1.toList == []
+#guard (runParserO (μ := List) concatParser "goodbye").1.toList == []
 -- #guard (runParser.{0} (μ := List) (concatParser ()) "hellogoodbye").1.toList == [(12, some (1, 2))]
 
 -- An ambiguous ε-free parser
-def concatParser2 [Monad μ] [Alternative μ] [Traversable μ] : Parser UChar μ PUnit :=
+def concatParser2 [CollectionLike μ] [Traversable μ] : Parser (tag := tag) UChar μ PUnit :=
   let p1 := terminal "a" <|> terminal "aa"
   p1 >>= fun _ => p1 $> PUnit.unit
 
 -- Ambiguity under Option vs. List
-#guard (runParser'.{0} (μ := Option) concatParser2 "").1.toList == []
-#guard (runParser'.{0} (μ := Option) concatParser2 "a").1.toList == []
-#guard (runParser'.{0} (μ := Option) concatParser2 "aa").1.toList == [(2, some PUnit.unit)]
-#guard (runParser'.{0} (μ := Option) concatParser2 "aaa").1.toList == [(2, some PUnit.unit), (3, some PUnit.unit)]
+#guard (runParserO (μ := Option) concatParser2 "").1.toList == []
+#guard (runParserO (μ := Option) concatParser2 "a").1.toList == []
+#guard (runParserO (μ := Option) concatParser2 "aa").1.toList == [(2, some PUnit.unit)]
+#guard (runParserO (μ := Option) concatParser2 "aaa").1.toList == [(2, some PUnit.unit), (3, some PUnit.unit)]
 
-#guard (runParser'.{0} (μ := List) concatParser2 "").1.toList == []
+#guard (runParserO (μ := List) concatParser2 "").1.toList == []
 -- NOTE(maemre): The code below crashes for some reason
 -- #eval (runParser.{0} (μ := List) concatParser2 "a").1.toList == []
 -- #eval (runParser.{0} (μ := List) concatParser2 "aa").1.toList
 
 @[inline]
-def concat [Monad μ] [Alternative μ] [Traversable μ] [Append α] (p₁ p₂ : Parser β μ α)
-    : Parser β μ α := liftA2 Append.append p₁ p₂
+def concat [CollectionLike μ] [Traversable μ] [Append α] (p₁ p₂ : Parser (tag := tag) β μ α)
+    : Parser (tag := tag) β μ α := liftA2 Append.append p₁ p₂
 
 instance [Append α] : Append (ULift α) where
   append a b := ULift.up $ a.down ++ b.down
 
 -- recursion via the inner parser function
-partial def recursiveParser [Monad μ] [Alternative μ] [Traversable μ] : Parser UChar μ UString :=
-  let p1 : Parser UChar μ UString := terminal "a"
-  let p2 : Parser UChar μ UString := terminal "b"
+partial def recursiveParser [CollectionLike μ] [Traversable μ] : Parser (tag := tag) UChar μ UString :=
+  let p1 : Parser (tag := tag) UChar μ UString := terminal "a"
+  let p2 : Parser (tag := tag) UChar μ UString := terminal "b"
   (concat p1 recursiveParser <|> p2)
 
-#guard (runParser'.{0} (μ := Option) recursiveParser "ab").1.toList == [(2, some $ ULift.up "ab")]
+#guard (runParserO (μ := Option) recursiveParser "ab").1.toList == [(2, some $ ULift.up "ab")]
 
 -- bounded recursion for a single parser
-def withFuel [Monad μ] [Alternative μ] [Traversable μ] (g : Parser β μ α → Parser β μ α) : ℕ → Parser β μ α
+def withFuel [CollectionLike μ] [Traversable μ] (g : Parser (tag := tag) β μ α → Parser (tag := tag) β μ α) : ℕ → Parser (tag := tag) β μ α
   | 0 => failure
   | Nat.succ fuel => g (withFuel g fuel)
 
-def fueledParser [Monad μ] [Alternative μ] [Traversable μ] : ℕ → Parser UChar μ UString := withFuel $ fun recur =>
-  let p1 : Parser UChar μ UString := terminal "a"
-  let p2 : Parser UChar μ UString := terminal "b"
+def fueledParser [CollectionLike μ] [Traversable μ] : ℕ → Parser (tag := tag) UChar μ UString := withFuel $ fun recur =>
+  let p1 : Parser (tag := tag) UChar μ UString := terminal "a"
+  let p2 : Parser (tag := tag) UChar μ UString := terminal "b"
   (concat p1 recur <|> p2)
 
-#guard (runParser'.{0} (μ := Option) (fueledParser 4) "aaab").1.toList = [(4, some { down := "aaab" })]
-#guard (runParser'.{0} (μ := Option) (fueledParser 3) "aaab").1.toList = []
+#guard (runParserO (μ := Option) (fueledParser 4) "aaab").1.toList = [(4, some { down := "aaab" })]
+#guard (runParserO (μ := Option) (fueledParser 3) "aaab").1.toList = []
 
 -- bounded recursion for parser families
-def withFuel' {τ} [Monad μ] [Alternative μ] [Traversable μ] (g : (τ → Parser β μ α) → τ → Parser β μ α) : ℕ → (t : τ) → Parser β μ α
+def withFuel' {τ'} [CollectionLike μ] [Traversable μ] (g : (τ' → Parser (tag := tag) β μ α) → τ' → Parser (tag := tag) β μ α) : ℕ → (t : τ') → Parser (tag := tag) β μ α
   | 0 => fun _ => failure
   | Nat.succ fuel => g (withFuel' g fuel)
 
@@ -260,22 +250,22 @@ X₁ -> b X₀
 
 X₀ =>⋆ (ab⋆)c
 -/
-def mutualRec : ℕ → Parser UChar Option UString := flip (withFuel' (τ := Fin 2) (fun recur t =>
+def mutualRec : ℕ → Parser (tag := tag) UChar Option UString := flip (withFuel' (τ' := Fin 2) $ fun recur t =>
   match t with
-  | 0 =>
-    -- A
-    concat (terminal "a") (recur 1) <|> terminal "c"
-  | 1 =>
-    -- B
-    concat (terminal "b") (recur 0)
-)) (0 : Fin 2)
+    | 0 =>
+      -- A
+      concat (terminal "a") (recur 1) <|> terminal "c"
+    | 1 =>
+      -- B
+      concat (terminal "b") (recur 0)
+  ) (0 : Fin 2)
 
-#guard (runParser'.{0} (mutualRec 5) "ababc").1.toList == [(5, some { down := "ababc" })]
-#guard (runParser'.{0} (mutualRec 4) "ababc").1.toList == []
+#guard (runParserO (mutualRec 5) "ababc").1.toList == [(5, some { down := "ababc" })]
+#guard (runParserO (mutualRec 4) "ababc").1.toList == []
 
 -- Induction theorem for bounded recursion
-theorem withFuel'_induction {τ} [Monad μ] [Alternative μ] [Traversable μ] {g : (τ → Parser β μ α) → τ → Parser β μ α}
-  {p : (τ → Parser β μ α) → Prop}
+theorem withFuel'_induction {τ} [CollectionLike μ] [Traversable μ] {g : (τ → Parser (tag := tag) β μ α) → τ → Parser (tag := tag) β μ α}
+  {p : (τ → Parser (tag := tag) β μ α) → Prop}
   (h_base : p (fun _ => failure))
   (h_recur : ∀ recur, p recur -> p (g recur))
   (n : ℕ)
@@ -288,24 +278,24 @@ theorem withFuel'_induction {τ} [Monad μ] [Alternative μ] [Traversable μ] {g
     exact h_recur (withFuel' g n') ih
 
 -- want something this:
-def memo [Monad μ] [Alternative μ] [Traversable μ] (g : Parser β μ α → Parser β μ α) : Parser β μ α :=
+def memo [CollectionLike μ] [Traversable μ] (g : Parser (tag := tag) β μ α → Parser (tag := tag) β μ α) : Parser (tag := tag) β μ α :=
   sorry
 
-def memo' {τ} [Monad μ] [Alternative μ] [Traversable μ] (g : (τ → Parser β μ α) → τ → Parser β μ α) : τ → Parser β μ α :=
+def memo' {τ} [CollectionLike μ] [Traversable μ] (g : (τ → Parser (tag := tag) β μ α) → τ → Parser (tag := tag) β μ α) : τ → Parser (tag := tag) β μ α :=
   sorry
 
 -- this just defines a subset-like relation on the parse results, the details of implementation
 -- aren't that crucial
-def subsumed [Monad μ] [Alternative μ] [Traversable μ] (a b : Std.HashMap Int (μ α)) : Prop :=
+def subsumed [CollectionLike μ] [Traversable μ] (a b : Std.HashMap Int (μ α)) : Prop :=
   ∀ k (h : k ∈ a), (a[k]'h <|> b[k]?.getD failure) = b[k]?.getD failure
 
 infix:50 " ≼ " => subsumed
 
 -- then, we want:
-theorem memo_sound [Monad μ] [Alternative μ] [Traversable μ] (g : Parser β μ α → Parser β μ α) n s
+theorem memo_sound [CollectionLike μ] [Traversable μ] (g : Parser (tag := tag) β μ α → Parser (tag := tag) β μ α) n s
     : (runParser (withFuel g n) s).1 ≼ (runParser (μ := μ) (memo g) s).1 := by
   sorry
 
-theorem memo_complete [Monad μ] [Alternative μ] [Traversable μ] (g : Parser β μ α → Parser β μ α) s
+theorem memo_complete [CollectionLike μ] [Traversable μ] (g : Parser (tag := tag) β μ α → Parser (tag := tag) β μ α) s
     : ∃ n, (runParser (μ := μ) (memo g) s).1 ≼ (runParser (withFuel g n) s).1 := by
   sorry
